Separate out multiple theory files

Launchbury.thy
@@ -1,512 +1,12 @@
 theory Launchbury
-  imports Main  "./Nominal/Nominal/Nominal2"
+imports Terms
 begin
 
-atom_decl var
-
-nominal_datatype exp =
-  Var "var"
-| App "exp" "var"
-| Let as::"assn" body::"exp" binds "bn as" in "body" "as"
-| Lam x::"var" body::"exp" binds x in body  ("Lam [_]. _" [100, 100] 100)
-and assn =
-  ANil | ACons "var" "exp" "assn" 
-binder
-  bn
-where "bn ANil = []" | "bn (ACons x t as) = (atom x) # (bn as)"
-
-fun subst_var :: "var \<Rightarrow> var \<Rightarrow> var \<Rightarrow> var" ("_[_::v=_]" [1000,100,100] 1000)
-where
- [simp]: "x[y ::v= z] = (if x = y then z else x)"
-
-lemma subst_var_eqvts[eqvt]:
- fixes \<pi>::perm
- shows "\<pi> \<bullet> (subst_var x y z) = subst_var (\<pi> \<bullet> x) (\<pi> \<bullet> y) (\<pi> \<bullet> z)"
-by auto
-
-type_synonym sum_type = "exp \<times> Launchbury.var \<times> Launchbury.var + assn \<times> Launchbury.var \<times> Launchbury.var \<Rightarrow> exp + assn"
-
-definition f1 ::
-    "(exp \<times> Launchbury.var \<times> Launchbury.var + assn \<times> Launchbury.var \<times> Launchbury.var \<Rightarrow> exp + assn \<Rightarrow> bool)
- \<Rightarrow> (exp \<times> Launchbury.var \<times> Launchbury.var + assn \<times> Launchbury.var \<times> Launchbury.var \<Rightarrow> exp + assn \<Rightarrow> bool)"
- where "f1 \<equiv>
- (\<lambda>p x1 x2.
-                (\<exists> (subst_subst_assn_sum :: sum_type)  x y z. x1 = Inl (Var x, y, z) \<and> x2 = Inl (Var x[y::v=z])) \<or>
-                (\<exists>(subst_subst_assn_sum :: sum_type) e v y z.
-                    x1 = Inl (App e v, y, z) \<and>
-                    x2 = Inl (App (Sum_Type.Projl (subst_subst_assn_sum (Inl (e, y, z)))) (v[y::v=z])) \<and>
-                    p (Inl (e, y, z)) (subst_subst_assn_sum (Inl (e, y, z)))) \<or>
-                (\<exists> (subst_subst_assn_sum :: sum_type)  as y z body.
-                    x1 = Inl (Launchbury.Let as body, y, z) \<and>
-                    x2 = Inl (Launchbury.Let (Sum_Type.Projr (subst_subst_assn_sum (Inr (as, y, z))))
-                               (Sum_Type.Projl (subst_subst_assn_sum (Inl (body, y, z))))) \<and>
-                    set (bn as) \<sharp>* (y, z) \<and>
-                    p (Inr (as, y, z)) (subst_subst_assn_sum (Inr (as, y, z))) \<and>
-                    p (Inl (body, y, z)) (subst_subst_assn_sum (Inl (body, y, z)))) \<or>
-                (\<exists>(subst_subst_assn_sum :: sum_type) x y z e.
-                    x1 = Inl (Lam [x]. e, y, z) \<and>
-                    x2 = Inl (Lam [x]. Sum_Type.Projl (subst_subst_assn_sum (Inl (e, y, z)))) \<and>
-                    atom x \<sharp> (y, z) \<and> p (Inl (e, y, z)) (subst_subst_assn_sum (Inl (e, y, z)))) \<or>
-                (\<exists>(subst_subst_assn_sum :: sum_type) y z. x1 = Inr (ANil, y, z) \<and> x2 = Inr ANil) \<or>
-                (\<exists>(subst_subst_assn_sum :: sum_type) v e as y z.
-                    x1 = Inr (ACons v e as, y, z) \<and>
-                    x2 = Inr (ACons v (Sum_Type.Projl (subst_subst_assn_sum (Inl (e, y, z))))
-                               (Sum_Type.Projr (subst_subst_assn_sum (Inr (as, y, z))))) \<and>
-                    p (Inl (e, y, z)) (subst_subst_assn_sum (Inl (e, y, z))) \<and> p (Inr (as, y, z)) (subst_subst_assn_sum (Inr (as, y, z)))))"
-
-definition f2 ::
-  "(exp \<times> Launchbury.var \<times> Launchbury.var + assn \<times> Launchbury.var \<times> Launchbury.var \<Rightarrow> exp + assn \<Rightarrow> bool)
- \<Rightarrow> (exp \<times> Launchbury.var \<times> Launchbury.var + assn \<times> Launchbury.var \<times> Launchbury.var \<Rightarrow> exp + assn \<Rightarrow> bool)"
-where "f2 \<equiv>
-(\<lambda>p x1 x2.
-                    (\<exists> x y z.
-                        x1 = Inl (Var x, y, z) \<and> x2 = Inl (Var (x[y::v=z]))) \<or>
-                    (\<exists>subst e v y z.
-                        x1 = Inl (App e v, y, z) \<and>
-                        x2 = Inl (App (subst (e, y, z)) (v[y::v=z])) \<and>
-                        p (Inl (e, y, z)) (Inl (subst (e, y, z)))) \<or>
-                    (\<exists>subst subst_assn as y z body.
-                        x1 = Inl (Launchbury.Let as body, y, z) \<and>
-                        x2 =
-                        Inl (Launchbury.Let
-                              (subst_assn (as, y, z))
-                              (subst (body, y, z))) \<and>
-                        set (bn as) \<sharp>* (y, z) \<and>
-                        p (Inr (as, y, z)) (Inr (subst_assn (as, y, z))) \<and>
-                        p (Inl (body, y, z)) (Inl (subst (body, y, z)))) \<or>
-                    (\<exists>subst x y z e.
-                        x1 = Inl (Lam [x]. e, y, z) \<and>
-                        x2 = Inl (Lam [x]. (subst (e, y, z))) \<and>
-                        atom x \<sharp> (y, z) \<and>
-                        p (Inl (e, y, z)) (Inl (subst (e, y, z)))) \<or>
-                    (\<exists> y z. x1 = Inr (ANil, y, z) \<and> x2 = Inr ANil) \<or>
-                    (\<exists>subst subst_assn as y z v e.
-                        x1 = Inr (ACons v e as, y, z) \<and>
-                        x2 =
-                        Inr (ACons v (subst (e, y, z))
-                              (subst_assn (as, y, z))) \<and>
-                        p (Inl (e, y, z)) (Inl (subst (e, y, z))) \<and>
-                        p (Inr (as, y, z)) (Inr (subst_assn (as, y, z)))))"
-
-
-ML {*
-fun mono_tac ctxt n =
- EVERY [rtac @{thm monoI} n,
-        REPEAT (resolve_tac [@{thm le_funI}, @{thm le_boolI'}] n),
-        REPEAT (FIRST
-         [atac n,
-          resolve_tac (Inductive.get_monos ctxt) n,
-          etac @{thm le_funE} n, 
-          dtac @{thm le_boolD} n])]
-*}
-
-lemma substAltDef:
-shows "lfp f1 = lfp f2"
-proof-
-
-have "mono f1" unfolding f1_def by (tactic {* mono_tac @{context} 1 *})
-have "mono f2" unfolding f2_def by (tactic {* mono_tac @{context} 1 *})
-
-show "lfp f1 = lfp f2"
-proof(rule antisym)
-  show "lfp f1 \<le> lfp f2"
-   apply(rule lfp_induct[OF `mono f1`])
-   apply(subst f1_def)
-   apply safe
-   apply (subst lfp_unfold[OF `mono f2`])
-   apply (subst f2_def)
-   apply auto[1]
-
-   apply (subst lfp_unfold[OF `mono f2`])
-   apply (subst (asm) lfp_unfold[OF `mono f1`])
-   apply (subst f2_def)
-   apply (subst (asm) f1_def)
-   apply auto[1]
-
-   apply (subst lfp_unfold[OF `mono f2`])
-   apply (subst f2_def)
-   apply auto[1]
-   apply (rule_tac x = "\<lambda>x . Sum_Type.Projl (subst_subst_assn_sum (Inl x))" in exI)
-   apply (rule_tac x = "\<lambda>x . Sum_Type.Projr (subst_subst_assn_sum (Inr x))" in exI)
-   apply (rule_tac x = "as" in exI)
-   apply (rule_tac x = "body" in exI)
-   apply auto[1]
-   apply (subst (asm) lfp_unfold[OF `mono f2`])
-   apply (subst (asm) f2_def)
-   apply auto[1]
-   apply (subst lfp_unfold[OF `mono f2`])
-   apply (subst f2_def)
-   apply auto[1]
-   apply (subst lfp_unfold[OF `mono f2`])
-   apply (subst f2_def)
-   apply auto[1]
-   apply (subst (asm) (2) lfp_unfold[OF `mono f1`])
-   apply (subst (asm) (2) f1_def)
-   apply auto[1]
-
-   apply (subst lfp_unfold[OF `mono f2`])
-   apply (subst f2_def)
-   apply auto[1]
-   apply (rule_tac x = "\<lambda>x . Sum_Type.Projl (subst_subst_assn_sum (Inl x))" in exI)
-   apply (rule_tac x = "xa" in exI)
-   apply (rule_tac x = "e" in exI)
-   apply auto[1]
-   apply (subst (asm) lfp_unfold[OF `mono f1`])
-   apply (subst (asm) f1_def)
-   apply auto[1]
-
-   
-   apply (subst lfp_unfold[OF `mono f2`])
-   apply (subst f2_def)
-   apply auto[1]
-
-   apply (subst lfp_unfold[OF `mono f2`])
-   apply (subst f2_def)
-   apply auto[1]
-   apply (rule_tac x = "\<lambda>x . Sum_Type.Projl (subst_subst_assn_sum (Inl x))" in exI)
-   apply auto[1]
-   apply (rule_tac x = "\<lambda>x . Sum_Type.Projr (subst_subst_assn_sum (Inr x))" in exI)
-   apply auto[1]
-   apply (subst (asm) lfp_unfold[OF `mono f1`])
-   apply (subst (asm) f1_def)
-   apply auto[1]
-   apply (subst (asm) (2) lfp_unfold[OF `mono f1`])
-   apply (subst (asm) (2) f1_def)
-   apply auto[1]
-   done
-next
-  show "lfp f2 \<le> lfp f1"
-  proof(rule lfp_mono)
-    fix p
-    show "f2 p \<le> f1 p"
-      unfolding f2_def f1_def
-      apply auto
-      apply (erule_tac x = "Inl \<circ> subst \<circ> Sum_Type.Projl" in allE, auto)
-      apply (erule_tac x = "Inl \<circ> subst \<circ> Sum_Type.Projl" in allE, auto)
-      apply (erule_tac x = "Inl \<circ> subst \<circ> Sum_Type.Projl" in allE, auto)
-      apply (erule_tac x = "Inl \<circ> subst \<circ> Sum_Type.Projl" in allE, auto)
-      apply (erule_tac x = "Inl \<circ> subst \<circ> Sum_Type.Projl" in allE, auto)
-      apply (erule_tac x = "Inl \<circ> subst \<circ> Sum_Type.Projl" in allE, auto)
-      apply (erule_tac x = "sum_case (Inl \<circ> subst) (Inr \<circ> subst_assn)" in allE, auto)
-      apply (erule_tac x = "sum_case (Inl \<circ> subst) (Inr \<circ> subst_assn)" in allE, auto)
-      apply (erule_tac x = "Inl \<circ> subst \<circ> Sum_Type.Projl" in allE, auto)
-      apply (erule_tac x = "Inl \<circ> subst \<circ> Sum_Type.Projl" in allE, auto)
-      apply (erule_tac x = "sum_case (Inl \<circ> subst) (Inr \<circ> subst_assn)" in allE, auto)
-      apply (erule_tac x = "sum_case (Inl \<circ> subst) (Inr \<circ> subst_assn)" in allE, auto)
-      done
-  qed
-qed
-qed
-
-(*
-Suggestion for a product-base fixed point, unused 
-
-definition f3 where
- "f3 \<equiv>(\<lambda> p .
-  ((\<lambda> x1 x2.
-                    (\<exists> x y z.
-                        x1 = (Var x, y, z) \<and> x2 = (Var (x[y::v=z]))) \<or>
-                    (\<exists>subst e v y z.
-                        x1 = (App e v, y, z) \<and>
-                        x2 = (App (subst (e, y, z)) (v[y::v=z])) \<and>
-                        fst p (e, y, z) (subst (e, y, z))) \<or>
-                    (\<exists>subst subst_assn as y z body.
-                        x1 = (Launchbury.Let as body, y, z) \<and>
-                        x2 = (Launchbury.Let
-                              (subst_assn (as, y, z))
-                              (subst (body, y, z))) \<and>
-                        set (bn as) \<sharp>* (y, z) \<and>
-                        snd p (as, y, z) (subst_assn (as, y, z)) \<and>
-                        fst p (body, y, z) (subst (body, y, z))) \<or>
-                    (\<exists>subst x y z e.
-                        x1 = (Lam [x]. e, y, z) \<and>
-                        x2 = (Lam [x]. (subst (e, y, z))) \<and>
-                        atom x \<sharp> (y, z) \<and>
-                        fst p ((e, y, z)) ((subst (e, y, z))))
-  ),(\<lambda> x1 x2.                     
-                    (\<exists> y z. x1 = (ANil, y, z) \<and> x2 = ANil) \<or>
-                    (\<exists>subst subst_assn as y z v e.
-                        x1 = (ACons v e as, y, z) \<and>
-                        x2 = (ACons v (subst (e, y, z)) (subst_assn (as, y, z))) \<and>
-                        fst p ((e, y, z)) ((subst (e, y, z))) \<and>
-                        snd p ((as, y, z)) ((subst_assn (as, y, z))))
-   ))
-)"
-
-
-definition conv where
-  "conv \<equiv> (\<lambda> fp. (\<lambda> x1 x2. sum_case (\<lambda> x1. sum_case (\<lambda> x2. fst fp x1 x2) (\<lambda> x2. False) x2) (\<lambda> x1. (sum_case (\<lambda> x2. False) (\<lambda> x2. snd fp x1 x2) x2)) x1))"
-
-lemma substAltEnc2:"
-lfp f2  = conv (lfp f3)"
-oops
-
-lemma sumC_rewrite:
- "(\<lambda>x. THE_default undefined (lfp f1 x)) = 
-  (sum_case (\<lambda>x1 . Inl (THE_default undefined (fst (lfp f3) x1)))
-            (\<lambda>x2 . Inr (THE_default undefined (snd (lfp f3) x2))))"
-oops
-*)
-
-(* Helper lemmas provided by Christian Urban *)
-
-lemma Projl_permute:
-  assumes a: "\<exists>y. f = Inl y"
-  shows "(p \<bullet> (Sum_Type.Projl f)) = Sum_Type.Projl (p \<bullet> f)"
-using a by auto
-
-lemma Projr_permute:
-  assumes a: "\<exists>y. f = Inr y"
-  shows "(p \<bullet> (Sum_Type.Projr f)) = Sum_Type.Projr (p \<bullet> f)"
-using a by auto
-
-nominal_primrec  (default "sum_case (\<lambda>x. Inl undefined) (\<lambda>x. Inr undefined)",
-                  invariant "\<lambda> a r . (\<forall> as y z . ((a = Inr (as, y, z) \<and> set (bn as) \<sharp>* (y, z)) \<longrightarrow> bn (Sum_Type.Projr r) = bn as))")
-  subst :: "exp \<Rightarrow> var \<Rightarrow> var \<Rightarrow> exp" ("_[_::=_]" [1000,100,100] 1000)
-and
-  subst_assn :: "assn \<Rightarrow> var \<Rightarrow> var \<Rightarrow> assn"
-where
-  "(Var x)[y ::= z] = (Var (x[y ::v= z]))"
- |"(App e v)[y ::= z] = (App (e[y ::= z]) (v[y ::v= z]))"
- |"(set (bn as)) \<sharp>* (y,z) \<Longrightarrow> (Let as body)[y ::= z] = Let (subst_assn as y z) (body[y ::= z])" 
- |"(atom x \<sharp> (y,z)) \<Longrightarrow> (Lam [x].e)[y ::= z] = Lam [x].(e[y::=z])"
- |"subst_assn ANil y z = ANil"
- |"subst_assn (ACons v e as) y z = ACons v (e[y ::= z]) (subst_assn as y z)"
-proof-
-
-have eqvt_at_subst: "\<And> e y z . eqvt_at subst_subst_assn_sumC (Inl (e, y, z)) \<Longrightarrow> eqvt_at (\<lambda>(a, b, c). subst a b c) (e, y, z)"
-  apply(simp add: eqvt_at_def subst_def)
-  apply(rule)
-  apply(subst Projl_permute)
-  apply(thin_tac "?X")+
-  apply (simp add: subst_subst_assn_sumC_def)
-  apply (simp add: THE_default_def)
-  apply (case_tac "Ex1 (subst_subst_assn_graph (Inl (e, y, z)))")
-  apply(simp)
-  apply(auto)[1]
-  apply (erule_tac x="x" in allE)
-  apply simp
-  apply(cases rule: subst_subst_assn_graph.cases)
-  apply(assumption)
-  apply(rule_tac x="Sum_Type.Projl x" in exI)
-  apply(clarify)
-  apply (rule the1_equality)
-  apply blast 
-  apply(simp (no_asm) only: Projl.simps)
-  apply(rule_tac x="Sum_Type.Projl x" in exI)
-  apply(clarify)
-  apply (rule the1_equality)
-  apply blast 
-  apply(simp (no_asm) only: Projl.simps)
-  apply(rule_tac x="Sum_Type.Projl x" in exI)
-  apply(clarify)
-  apply (rule the1_equality)
-  apply blast 
-  apply(simp (no_asm) only: Projl.simps)
-  apply(rule_tac x="Sum_Type.Projl x" in exI)
-  apply(clarify)
-  apply (rule the1_equality)
-  apply blast 
-  apply(simp (no_asm) only: Projl.simps)
-  apply (metis Inr_not_Inl)
-  apply (metis Inr_not_Inl)
-  apply(simp)
-  apply(perm_simp)
-  apply(simp)
-done
-
-have eqvt_at_subst_assn: "\<And> as y z . eqvt_at subst_subst_assn_sumC (Inr (as, y, z)) \<Longrightarrow> eqvt_at (\<lambda>(a, b, c). subst_assn a b c) (as, y, z)"
-  apply(simp add: eqvt_at_def subst_assn_def)
-  apply(rule)
-  apply(subst Projr_permute)
-  apply(thin_tac "?X")+
-  apply (simp add: subst_subst_assn_sumC_def)
-  apply (simp add: THE_default_def)
-  apply (case_tac "Ex1 (subst_subst_assn_graph (Inr (as, y, z)))")
-  apply(simp)
-  apply(auto)[1]
-  apply (erule_tac x="x" in allE)
-  apply simp
-  apply(cases rule: subst_subst_assn_graph.cases)
-  apply(assumption)
-  apply (metis Inr_not_Inl)+
-  apply(rule_tac x="Sum_Type.Projr x" in exI)
-  apply(clarify)
-  apply (rule the1_equality)
-  apply auto[1]
-  apply(simp (no_asm) only: Projr.simps)
-  
-  apply(rule_tac x="Sum_Type.Projr x" in exI)
-  apply(clarify)
-  apply (rule the1_equality)
-  apply auto[1]
-  apply(simp (no_asm) only: Projr.simps)
-  
-  apply(simp)
-  apply(perm_simp)
-  apply(simp)
-done
-
-{
-(* Equivariance of the graph *)
-case goal1 thus ?case
-  unfolding eqvt_def subst_subst_assn_graph_def
-  apply(subst (1 2) substAltDef[unfolded f1_def f2_def]) 
-  apply(rule)
-  apply perm_simp
-  apply rule
-done
-
-(* The invariant *)
-next case goal2 thus ?case
-  by (induct rule: subst_subst_assn_graph.induct)(auto simp add: exp_assn.bn_defs fresh_star_insert)
-
-(* Exhaustiveness *)
-next case (goal3 P x) show ?case
-  proof(cases x)
-  case (Inl a) thus P
-    proof(cases a)
-    case (fields a1 a2 a3)
-    thus P using Inl goal3
-      apply (rule_tac y ="a1" and c ="(a2, a3)" in exp_assn.strong_exhaust(1))
-      apply (auto simp add: fresh_star_def)
-    done
-  qed
-  next
-  case (Inr a) thus P
-    proof (cases a)
-    case (fields a1 a2 a3)
-    thus P using Inr goal3
-      apply (rule_tac ya ="a1" in exp_assn.strong_exhaust(2))
-      apply (auto)
-      apply blast+
-    done
-  qed
-qed
-
-next case (goal15 e y2 z2 as e2 y z as2) thus ?case
-  apply -
-  apply (drule eqvt_at_subst)+
-  apply (drule eqvt_at_subst_assn)+
-  apply (simp only: meta_eq_to_obj_eq[OF subst_def, symmetric, unfolded fun_eq_iff]
-    meta_eq_to_obj_eq[OF subst_assn_def, symmetric, unfolded fun_eq_iff])
-  (* No _sum any more at this point! *)
-  apply (auto simp add: Abs_fresh_iff)
-  apply (drule_tac
-    c = "(y, z)" and
-    as = "(bn e)" and
-    bs = "(bn e2)" and
-    f = "\<lambda> a b c . [a]lst. (subst (fst b) y z, subst_assn (snd b) y z )" in Abs_lst_fcb2)
-  apply (auto simp add: perm_supp_eq fresh_Pair fresh_star_def Abs_fresh_iff eqvt_at_def)
-  done
-
-next case (goal19 x2 y2 z2 e2 x y z e) thus ?case
-  apply -
-  apply (drule eqvt_at_subst)+
-  apply (simp only: Abs_fresh_iff meta_eq_to_obj_eq[OF subst_def, symmetric, unfolded fun_eq_iff])
-  (* No _sum any more at this point! *)
-  apply (auto)
-  apply (erule_tac c = "(y, z)" in Abs_lst_fcb2)
-  apply (auto simp add: perm_supp_eq fresh_Pair fresh_star_def Abs_fresh_iff eqvt_at_def)
-  done
-}
-qed(auto)
-
-termination (eqvt) by lexicographic_order
-
-lemma shows
-  True and bn_subst[simp]: "set (bn as) \<sharp>* (y, z) \<Longrightarrow> bn (subst_assn as y z) = bn as"
-by(induct rule:subst_subst_assn.induct)
-  (auto simp add: exp_assn.bn_defs fresh_star_insert)
-
-abbreviation
-  LetBe :: "var\<Rightarrow>exp\<Rightarrow>exp\<Rightarrow>exp" ("let _ be _ in _ " [100,100,100] 100)
-where
-  "let x be t1 in t2 \<equiv> Let (ACons x t1 ANil) t2"
-              
-lemma alpha_test:
-  shows "Lam [x]. (Var x) = Lam [y]. (Var y)"
-  by (simp add: exp_assn.eq_iff Abs1_eq_iff exp_assn.fresh fresh_at_base)
-
-lemma alpha_test2:
-  shows "let x be (Var x) in (Var x) = let y be (Var y) in (Var y)"
-  by (simp add:exp_assn.eq_iff exp_assn.bn_defs Abs1_eq_iff fresh_Pair add:exp_assn.fresh fresh_at_base)
-
-lemma alpha_test3:
-  shows "
-    Let (ACons x (Var y) (ACons y (Var x) ANil)) (Var x)
-    =
-    Let (ACons y (Var x) (ACons x (Var y) ANil)) (Var y)" (is "Let ?la ?lb = _")
-  apply (simp add:exp_assn.eq_iff exp_assn.bn_defs Abs1_eq_iff fresh_Pair add:exp_assn.fresh fresh_at_base)
-  apply (simp add: Abs_swap2[of "atom x" "(?lb,?la)" "[atom x, atom y]" "atom y"])
-done
-
-
-(* type_synonym heap = "(var \<times> exp) list" *)
-
-nominal_datatype 
-heapexp = Heap heap::heap body::exp binds "hbn heap" in heap body
-and
-heap =  HNil | HCons var exp heap ("'(_ \<mapsto> _') ## _" [65,65,65] 65)
-binder
-  hbn
-where "hbn HNil = []" | "hbn (HCons x t h) = (atom x) # (hbn h)"
-
-function elemLookup :: "heap \<Rightarrow> var \<Rightarrow> exp option" (infix "\<cdot>" 62)
-  where
-    "HNil \<cdot> x = None"
-    | "(v \<mapsto> e) ## h \<cdot> x = (if x = v then Some e else h \<cdot> x)"
-apply(case_tac x)
-apply(case_tac a rule: heapexp_heap.exhaust(2))
-apply auto
-done
-termination by lexicographic_order
-
-lemma elemLookup_eqvt[eqvt]:
- fixes \<pi>::perm
- shows "\<pi> \<bullet> (h \<cdot> x) = (\<pi> \<bullet> h) \<cdot> (\<pi> \<bullet> x)"
-by(induct h x rule:elemLookup.induct) (auto simp add:elemLookup.simps)
-
-
-function removeHeap :: "heap \<Rightarrow> var \<Rightarrow> heap" ("_ with _ removed" [80,80] 80)
-where "HNil with x removed = HNil"
-| "((v \<mapsto> e) ## h) with x removed = (if v = x then h with x removed else (v \<mapsto> e) ## h with x removed)"
-apply(case_tac x)
-apply(case_tac a rule: heapexp_heap.exhaust(2))
-apply auto
-done
-termination by lexicographic_order
-
-lemma removeHeap_eqvt[eqvt]:
- fixes \<pi>::perm
- shows "\<pi> \<bullet> (removeHeap x y) = removeHeap (\<pi> \<bullet> x) (\<pi> \<bullet> y)"
-by(induct x y rule:removeHeap.induct) (auto simp add:removeHeap.simps)
-
-
-inductive reds :: "heap \<Rightarrow> exp \<Rightarrow> heap \<Rightarrow> exp \<Rightarrow> bool" ("_ : _ \<Down> _ : _" [50,50,50,50] 50)
-where
-  Lambda: "\<Gamma> : (Lam [x]. e) \<Down> \<Gamma> : (Lam [x]. e)" 
- | Application: "\<lbrakk>  \<Gamma> : e \<Down> \<Delta> : (Lam [y]. e') ; \<Delta> : e'[y ::= x] \<Down> \<Theta> : z\<rbrakk> \<Longrightarrow> \<Gamma> : App e x \<Down> \<Theta> : z" 
- | Variable: "\<lbrakk>\<Gamma> \<cdot> x = Some e; \<Gamma> with x removed : e \<Down> \<Delta> : z \<rbrakk> \<Longrightarrow> \<Gamma> : Var x \<Down> (x \<mapsto> z) ## \<Delta> : z"
- | LetANil: "\<Gamma> : body \<Down> \<Delta> : z \<Longrightarrow> \<Gamma> : (Let ANil body) \<Down> \<Delta> : z"
- | LetACons: "(v \<mapsto> e) ## \<Gamma> : Let as body \<Down> \<Delta> : z \<Longrightarrow> \<Gamma> : (Let (ACons v e as) body) \<Down> \<Delta> : z"
+type_synonym heap = "(var \<times> exp) list"
 
 
 lemma fun_upd[eqvt]: "p \<bullet> (fun_upd f x y) = fun_upd (p \<bullet> f) (p \<bullet> x) (p \<bullet> y)"
 by  (auto simp add:permute_fun_def fun_eq_iff)
-
-equivariance reds
-
-nominal_inductive reds .
-(*
-  avoids Application: "y"
-apply (auto simp add: fresh_star_def fresh_Pair exp_assn.fresh)
-*)
-
-
-lemma eval_test:
-  "HNil : (Let (ACons x (Lam [y]. Var y) ANil) (Var x)) \<Down> (x \<mapsto> Lam [y]. Var y) ## HNil : (Lam [y]. Var y)"
-by (auto intro!: Lambda Application Variable LetANil LetACons)
 
 lemma fresh_upd[intro]:
   assumes "atom x \<sharp> \<Gamma>(y := None)" and "atom x \<sharp> e"
@@ -526,30 +26,12 @@ lemma fresh_remove:
 using assms
 by(induct \<Gamma>)(auto simp add: fresh_Cons)
 
-lemma fresh_removeHeap:
-  assumes "atom x \<sharp> \<Gamma>"
-  shows "atom x \<sharp> \<Gamma> with v removed"
-using assms
-by(induct \<Gamma> v rule:removeHeap.induct)(auto simp add: heapexp_heap.fresh)
-
 lemma fresh_list_elem:
   assumes "atom x \<sharp> \<Gamma>"
   and "e \<in> set \<Gamma>"
   shows "atom x \<sharp> e"
 using assms
 by(induct \<Gamma>)(auto simp add: fresh_Cons)
-
-lemma fresh_heap_elem:
-  assumes "atom x \<sharp> \<Gamma>"
-  and "\<Gamma> \<cdot> v = Some e"
-  shows "atom x \<sharp> e"
-using assms
-by(induct \<Gamma> v rule:elemLookup.induct)(auto simp add: heapexp_heap.fresh split_if_eq1)
-
-
-lemma eval_test2:
-  "HNil : (Let (ACons x (Lam [y]. Var y) ANil) (App (Var x) x)) \<Down> (x \<mapsto> Lam [y]. Var y) ## HNil : (Lam [y]. Var y)"
-by (auto intro!: Lambda Application Variable LetANil LetACons)
 
 lemma subst_is_fresh:
 assumes "atom y \<sharp> z"
@@ -569,15 +51,49 @@ and
 by(induct e y z and as y z rule:subst_subst_assn.induct)
   (auto simp add:exp_assn.fresh fresh_at_base fresh_star_Pair exp_assn.bn_defs fresh_star_insert)
 
-lemma reds_fresh:"\<lbrakk> \<Gamma> : e \<Down> \<Delta> : z ; atom (x::var) \<sharp> (\<Gamma>, e) \<rbrakk> \<Longrightarrow> atom x \<sharp> (\<Delta>, z)"
-thm reds.induct
-thm reds.strong_induct
-proof(induct rule: reds.induct)
-print_cases
 
+inductive reds :: "heap \<Rightarrow> exp \<Rightarrow> heap \<Rightarrow> exp \<Rightarrow> bool" ("_ : _ \<Down> _ : _" [50,50,50,50] 50)
+where
+  Lambda: "\<Gamma> : (Lam [x]. e) \<Down> \<Gamma> : (Lam [x]. e)" 
+ | Application: "\<lbrakk>  \<Gamma> : e \<Down> \<Delta> : (Lam [y]. e') ; \<Delta> : e'[y ::= x] \<Down> \<Theta> : z\<rbrakk> \<Longrightarrow> \<Gamma> : App e x \<Down> \<Theta> : z" 
+ | Variable: "\<lbrakk> (x,e) \<in> set \<Gamma>; removeAll (x, e) \<Gamma> : e \<Down> \<Delta> : z \<rbrakk> \<Longrightarrow> \<Gamma> : Var x \<Down> (x, z) # \<Delta> : z"
+ | LetANil: "\<Gamma> : body \<Down> \<Delta> : z \<Longrightarrow> \<Gamma> : (Let ANil body) \<Down> \<Delta> : z"
+ | LetACons: "\<lbrakk>  (v, e) # \<Gamma> : Let as body \<Down> \<Delta> : z \<rbrakk> \<Longrightarrow> \<Gamma> : (Let (ACons v e as) body) \<Down> \<Delta> : z"
+
+equivariance reds
+
+nominal_inductive reds.
+(*
+  avoids LetACons: "v"
+apply (auto simp add: fresh_star_def fresh_Pair exp_assn.fresh exp_assn.bn_defs)
+done
+*)
+(*
+  avoids Application: "y"
+apply (auto simp add: fresh_star_def fresh_Pair exp_assn.fresh)
+*)
+
+lemma eval_test:
+  "[] : (Let (ACons x (Lam [y]. Var y) ANil) (Var x)) \<Down> [(x, Lam [y]. Var y)] : (Lam [y]. Var y)"
+apply(auto intro!: Lambda Application Variable LetANil LetACons
+ simp add: fresh_Pair fresh_Cons fresh_Nil exp_assn.fresh)
+done
+
+lemma eval_test2:
+  "[] : (Let (ACons x (Lam [y]. Var y) ANil) (App (Var x) x)) \<Down> [(x, Lam [y]. Var y)] : (Lam [y]. Var y)"
+by (auto intro!: Lambda Application Variable LetANil LetACons)
+
+lemma reds_fresh:"
+  \<lbrakk> \<Gamma> : e \<Down> \<Delta> : z;
+  atom (x::var) \<sharp> (\<Gamma>, e);
+  x \<notin> fst ` (set \<Gamma>)
+  \<rbrakk> \<Longrightarrow> (atom x \<sharp> (\<Delta>, z) \<and> x \<notin> fst ` (set \<Delta>))"
+proof(induct rule: reds.induct)
+case (Lambda \<Gamma> x e) thus ?case ..
+next
 case (Application \<Gamma> e \<Delta> y e' x' \<Theta> z)
-  have "atom x \<sharp> \<Gamma>" "atom x \<sharp> e" "atom x \<sharp> x'" using Application.prems by (auto simp add: exp_assn.fresh fresh_Pair)  
-  hence "atom x \<sharp> \<Delta>" "atom x \<sharp> (Lam [y]. e')" using Application.hyps(2)  by auto
+  have "atom x \<sharp> \<Gamma>" "atom x \<sharp> e" "atom x \<sharp> x'" using Application.prems(1) by (auto simp add: exp_assn.fresh fresh_Pair)  
+  hence "atom x \<sharp> \<Delta>" "atom x \<sharp> (Lam [y]. e')" "x \<notin> fst ` (set \<Delta>) " using Application.hyps(2) Application.prems(2) by auto
   show ?case
   proof(cases "x = y")
     case False
@@ -586,20 +102,20 @@ case (Application \<Gamma> e \<Delta> y e' x' \<Theta> z)
       *)
       hence "atom x \<sharp> e'" using `atom x \<sharp> (Lam [y]. e')` by (auto simp add: exp_assn.fresh)
       hence "atom x \<sharp> e'[y ::= x']" using `atom x \<sharp> x'` by (auto intro: subst_pres_fresh[rule_format])
-      thus "atom x \<sharp> (\<Theta>, z)" using Application.hyps(4) `atom x \<sharp> \<Delta>` by auto
+      thus ?thesis using Application.hyps(4) `atom x \<sharp> \<Delta>` `x \<notin> fst \` (set \<Delta>)` by auto
     next
     case True
       hence "atom x \<sharp> e'[y ::= x']" using  `atom x \<sharp> x'` by (auto intro: subst_is_fresh)
-      thus "atom x \<sharp> (\<Theta>, z)" using Application.hyps(4) `atom x \<sharp> \<Delta>` by auto
+      thus ?thesis using Application.hyps(4) `atom x \<sharp> \<Delta>` `x \<notin> fst \` (set \<Delta>)` by auto
   qed
 next
 
-case(Variable \<Gamma> v e \<Delta> z)
+case(Variable v e \<Gamma> \<Delta> z)
   print_facts
-  have "atom x \<sharp> \<Gamma>" and "atom x \<sharp> v" using Variable.prems by (auto simp add: fresh_Pair exp_assn.fresh)
-  hence "atom x \<sharp> \<Gamma> with v removed" and "atom x \<sharp> e" using `\<Gamma> \<cdot> v = Some e` by(auto intro: fresh_removeHeap dest:fresh_heap_elem)
-  hence "atom x \<sharp> (\<Delta>, z)" using Variable.hyps(3) by (auto simp add: fresh_Pair)
-  thus "atom x \<sharp> ((v \<mapsto> z) ## \<Delta>, z)" using `atom x \<sharp> (\<Delta>, z)` `atom x \<sharp> v` by (auto simp add: fresh_Pair heapexp_heap.fresh)
+  have "atom x \<sharp> \<Gamma>" and "atom x \<sharp> v" using Variable.prems(1) by (auto simp add: fresh_Pair exp_assn.fresh)
+  hence "atom x \<sharp> removeAll (v,e) \<Gamma>" and "atom x \<sharp> e" using `(v,e) \<in> set \<Gamma>` by(auto intro: fresh_remove dest:fresh_list_elem)
+  hence "atom x \<sharp> (\<Delta>, z)" and "x \<notin> fst ` (set \<Delta>)" using Variable.hyps(3) Variable.prems(2) by (auto simp add: fresh_Pair)
+  thus ?case using `atom x \<sharp> v` by (auto simp add: fresh_Pair fresh_Cons fresh_at_base)
 next
 
 case(LetANil \<Gamma> body \<Delta> z)
@@ -617,13 +133,15 @@ case(LetACons v e \<Gamma> as body \<Delta> z)
         using `atom x \<sharp> Let (ACons v e as) body`
         by (auto simp add: exp_assn.fresh exp_assn.bn_defs)
       thus ?thesis
-        using `atom x \<sharp> \<Gamma>` and LetACons.hyps(2)
-        by (auto simp add: fresh_Pair heapexp_heap.fresh exp_assn.fresh)
+        apply -
+        apply (rule LetACons.hyps(2))
+        using `atom x \<sharp> \<Gamma>` and LetACons.prems(2)
+        by (auto simp add: fresh_Pair fresh_Cons  exp_assn.fresh fresh_at_base)
     next
     case True
       print_facts
-
-
+      show ?thesis sorry
+    qed
 qed
 
 end
