Terms.thy
@@ -1,0 +1,488 @@
+theory Terms
+  imports Main  "./Nominal/Nominal/Nominal2"
+begin
+
+atom_decl var
+
+nominal_datatype exp =
+  Var "var"
+| App "exp" "var"
+| Let as::"assn" body::"exp" binds "bn as" in "body" "as"
+| Lam x::"var" body::"exp" binds x in body  ("Lam [_]. _" [100, 100] 100)
+and assn =
+  ANil | ACons "var" "exp" "assn" 
+binder
+  bn
+where "bn ANil = []" | "bn (ACons x t as) = (atom x) # (bn as)"
+
+fun subst_var :: "var \<Rightarrow> var \<Rightarrow> var \<Rightarrow> var" ("_[_::v=_]" [1000,100,100] 1000)
+where
+ [simp]: "x[y ::v= z] = (if x = y then z else x)"
+
+lemma subst_var_eqvts[eqvt]:
+ fixes \<pi>::perm
+ shows "\<pi> \<bullet> (subst_var x y z) = subst_var (\<pi> \<bullet> x) (\<pi> \<bullet> y) (\<pi> \<bullet> z)"
+by auto
+
+type_synonym sum_type = "exp \<times> var \<times> var + assn \<times> var \<times> var \<Rightarrow> exp + assn"
+
+definition f1 ::
+    "(exp \<times> var \<times> var + assn \<times> var \<times> var \<Rightarrow> exp + assn \<Rightarrow> bool)
+ \<Rightarrow> (exp \<times> var \<times> var + assn \<times> var \<times> var \<Rightarrow> exp + assn \<Rightarrow> bool)"
+ where "f1 \<equiv>
+ (\<lambda>p x1 x2.
+                (\<exists> (subst_subst_assn_sum :: sum_type)  x y z. x1 = Inl (Var x, y, z) \<and> x2 = Inl (Var x[y::v=z])) \<or>
+                (\<exists>(subst_subst_assn_sum :: sum_type) e v y z.
+                    x1 = Inl (App e v, y, z) \<and>
+                    x2 = Inl (App (Sum_Type.Projl (subst_subst_assn_sum (Inl (e, y, z)))) (v[y::v=z])) \<and>
+                    p (Inl (e, y, z)) (subst_subst_assn_sum (Inl (e, y, z)))) \<or>
+                (\<exists> (subst_subst_assn_sum :: sum_type)  as y z body.
+                    x1 = Inl (Let as body, y, z) \<and>
+                    x2 = Inl (Let (Sum_Type.Projr (subst_subst_assn_sum (Inr (as, y, z))))
+                               (Sum_Type.Projl (subst_subst_assn_sum (Inl (body, y, z))))) \<and>
+                    set (bn as) \<sharp>* (y, z) \<and>
+                    p (Inr (as, y, z)) (subst_subst_assn_sum (Inr (as, y, z))) \<and>
+                    p (Inl (body, y, z)) (subst_subst_assn_sum (Inl (body, y, z)))) \<or>
+                (\<exists>(subst_subst_assn_sum :: sum_type) x y z e.
+                    x1 = Inl (Lam [x]. e, y, z) \<and>
+                    x2 = Inl (Lam [x]. Sum_Type.Projl (subst_subst_assn_sum (Inl (e, y, z)))) \<and>
+                    atom x \<sharp> (y, z) \<and> p (Inl (e, y, z)) (subst_subst_assn_sum (Inl (e, y, z)))) \<or>
+                (\<exists>(subst_subst_assn_sum :: sum_type) y z. x1 = Inr (ANil, y, z) \<and> x2 = Inr ANil) \<or>
+                (\<exists>(subst_subst_assn_sum :: sum_type) v e as y z.
+                    x1 = Inr (ACons v e as, y, z) \<and>
+                    x2 = Inr (ACons v (Sum_Type.Projl (subst_subst_assn_sum (Inl (e, y, z))))
+                               (Sum_Type.Projr (subst_subst_assn_sum (Inr (as, y, z))))) \<and>
+                    p (Inl (e, y, z)) (subst_subst_assn_sum (Inl (e, y, z))) \<and> p (Inr (as, y, z)) (subst_subst_assn_sum (Inr (as, y, z)))))"
+
+definition f2 ::
+  "(exp \<times> var \<times> var + assn \<times> var \<times> var \<Rightarrow> exp + assn \<Rightarrow> bool)
+ \<Rightarrow> (exp \<times> var \<times> var + assn \<times> var \<times> var \<Rightarrow> exp + assn \<Rightarrow> bool)"
+where "f2 \<equiv>
+(\<lambda>p x1 x2.
+                    (\<exists> x y z.
+                        x1 = Inl (Var x, y, z) \<and> x2 = Inl (Var (x[y::v=z]))) \<or>
+                    (\<exists>subst e v y z.
+                        x1 = Inl (App e v, y, z) \<and>
+                        x2 = Inl (App (subst (e, y, z)) (v[y::v=z])) \<and>
+                        p (Inl (e, y, z)) (Inl (subst (e, y, z)))) \<or>
+                    (\<exists>subst subst_assn as y z body.
+                        x1 = Inl (Let as body, y, z) \<and>
+                        x2 =
+                        Inl (Let
+                              (subst_assn (as, y, z))
+                              (subst (body, y, z))) \<and>
+                        set (bn as) \<sharp>* (y, z) \<and>
+                        p (Inr (as, y, z)) (Inr (subst_assn (as, y, z))) \<and>
+                        p (Inl (body, y, z)) (Inl (subst (body, y, z)))) \<or>
+                    (\<exists>subst x y z e.
+                        x1 = Inl (Lam [x]. e, y, z) \<and>
+                        x2 = Inl (Lam [x]. (subst (e, y, z))) \<and>
+                        atom x \<sharp> (y, z) \<and>
+                        p (Inl (e, y, z)) (Inl (subst (e, y, z)))) \<or>
+                    (\<exists> y z. x1 = Inr (ANil, y, z) \<and> x2 = Inr ANil) \<or>
+                    (\<exists>subst subst_assn as y z v e.
+                        x1 = Inr (ACons v e as, y, z) \<and>
+                        x2 =
+                        Inr (ACons v (subst (e, y, z))
+                              (subst_assn (as, y, z))) \<and>
+                        p (Inl (e, y, z)) (Inl (subst (e, y, z))) \<and>
+                        p (Inr (as, y, z)) (Inr (subst_assn (as, y, z)))))"
+
+
+ML {*
+fun mono_tac ctxt n =
+ EVERY [rtac @{thm monoI} n,
+        REPEAT (resolve_tac [@{thm le_funI}, @{thm le_boolI'}] n),
+        REPEAT (FIRST
+         [atac n,
+          resolve_tac (Inductive.get_monos ctxt) n,
+          etac @{thm le_funE} n, 
+          dtac @{thm le_boolD} n])]
+*}
+
+lemma substAltDef:
+shows "lfp f1 = lfp f2"
+proof-
+
+have "mono f1" unfolding f1_def by (tactic {* mono_tac @{context} 1 *})
+have "mono f2" unfolding f2_def by (tactic {* mono_tac @{context} 1 *})
+
+show "lfp f1 = lfp f2"
+proof(rule antisym)
+  show "lfp f1 \<le> lfp f2"
+   apply(rule lfp_induct[OF `mono f1`])
+   apply(subst f1_def)
+   apply safe
+   apply (subst lfp_unfold[OF `mono f2`])
+   apply (subst f2_def)
+   apply auto[1]
+
+   apply (subst lfp_unfold[OF `mono f2`])
+   apply (subst (asm) lfp_unfold[OF `mono f1`])
+   apply (subst f2_def)
+   apply (subst (asm) f1_def)
+   apply auto[1]
+
+   apply (subst lfp_unfold[OF `mono f2`])
+   apply (subst f2_def)
+   apply auto[1]
+   apply (rule_tac x = "\<lambda>x . Sum_Type.Projl (subst_subst_assn_sum (Inl x))" in exI)
+   apply (rule_tac x = "\<lambda>x . Sum_Type.Projr (subst_subst_assn_sum (Inr x))" in exI)
+   apply (rule_tac x = "as" in exI)
+   apply (rule_tac x = "body" in exI)
+   apply auto[1]
+   apply (subst (asm) lfp_unfold[OF `mono f2`])
+   apply (subst (asm) f2_def)
+   apply auto[1]
+   apply (subst lfp_unfold[OF `mono f2`])
+   apply (subst f2_def)
+   apply auto[1]
+   apply (subst lfp_unfold[OF `mono f2`])
+   apply (subst f2_def)
+   apply auto[1]
+   apply (subst (asm) (2) lfp_unfold[OF `mono f1`])
+   apply (subst (asm) (2) f1_def)
+   apply auto[1]
+
+   apply (subst lfp_unfold[OF `mono f2`])
+   apply (subst f2_def)
+   apply auto[1]
+   apply (rule_tac x = "\<lambda>x . Sum_Type.Projl (subst_subst_assn_sum (Inl x))" in exI)
+   apply (rule_tac x = "xa" in exI)
+   apply (rule_tac x = "e" in exI)
+   apply auto[1]
+   apply (subst (asm) lfp_unfold[OF `mono f1`])
+   apply (subst (asm) f1_def)
+   apply auto[1]
+
+   
+   apply (subst lfp_unfold[OF `mono f2`])
+   apply (subst f2_def)
+   apply auto[1]
+
+   apply (subst lfp_unfold[OF `mono f2`])
+   apply (subst f2_def)
+   apply auto[1]
+   apply (rule_tac x = "\<lambda>x . Sum_Type.Projl (subst_subst_assn_sum (Inl x))" in exI)
+   apply auto[1]
+   apply (rule_tac x = "\<lambda>x . Sum_Type.Projr (subst_subst_assn_sum (Inr x))" in exI)
+   apply auto[1]
+   apply (subst (asm) lfp_unfold[OF `mono f1`])
+   apply (subst (asm) f1_def)
+   apply auto[1]
+   apply (subst (asm) (2) lfp_unfold[OF `mono f1`])
+   apply (subst (asm) (2) f1_def)
+   apply auto[1]
+   done
+next
+  show "lfp f2 \<le> lfp f1"
+  proof(rule lfp_mono)
+    fix p
+    show "f2 p \<le> f1 p"
+      unfolding f2_def f1_def
+      apply auto
+      apply (erule_tac x = "Inl \<circ> subst \<circ> Sum_Type.Projl" in allE, auto)
+      apply (erule_tac x = "Inl \<circ> subst \<circ> Sum_Type.Projl" in allE, auto)
+      apply (erule_tac x = "Inl \<circ> subst \<circ> Sum_Type.Projl" in allE, auto)
+      apply (erule_tac x = "Inl \<circ> subst \<circ> Sum_Type.Projl" in allE, auto)
+      apply (erule_tac x = "Inl \<circ> subst \<circ> Sum_Type.Projl" in allE, auto)
+      apply (erule_tac x = "Inl \<circ> subst \<circ> Sum_Type.Projl" in allE, auto)
+      apply (erule_tac x = "sum_case (Inl \<circ> subst) (Inr \<circ> subst_assn)" in allE, auto)
+      apply (erule_tac x = "sum_case (Inl \<circ> subst) (Inr \<circ> subst_assn)" in allE, auto)
+      apply (erule_tac x = "Inl \<circ> subst \<circ> Sum_Type.Projl" in allE, auto)
+      apply (erule_tac x = "Inl \<circ> subst \<circ> Sum_Type.Projl" in allE, auto)
+      apply (erule_tac x = "sum_case (Inl \<circ> subst) (Inr \<circ> subst_assn)" in allE, auto)
+      apply (erule_tac x = "sum_case (Inl \<circ> subst) (Inr \<circ> subst_assn)" in allE, auto)
+      done
+  qed
+qed
+qed
+
+(*
+Suggestion for a product-base fixed point, unused 
+
+definition f3 where
+ "f3 \<equiv>(\<lambda> p .
+  ((\<lambda> x1 x2.
+                    (\<exists> x y z.
+                        x1 = (Var x, y, z) \<and> x2 = (Var (x[y::v=z]))) \<or>
+                    (\<exists>subst e v y z.
+                        x1 = (App e v, y, z) \<and>
+                        x2 = (App (subst (e, y, z)) (v[y::v=z])) \<and>
+                        fst p (e, y, z) (subst (e, y, z))) \<or>
+                    (\<exists>subst subst_assn as y z body.
+                        x1 = (Launchbury.Let as body, y, z) \<and>
+                        x2 = (Launchbury.Let
+                              (subst_assn (as, y, z))
+                              (subst (body, y, z))) \<and>
+                        set (bn as) \<sharp>* (y, z) \<and>
+                        snd p (as, y, z) (subst_assn (as, y, z)) \<and>
+                        fst p (body, y, z) (subst (body, y, z))) \<or>
+                    (\<exists>subst x y z e.
+                        x1 = (Lam [x]. e, y, z) \<and>
+                        x2 = (Lam [x]. (subst (e, y, z))) \<and>
+                        atom x \<sharp> (y, z) \<and>
+                        fst p ((e, y, z)) ((subst (e, y, z))))
+  ),(\<lambda> x1 x2.                     
+                    (\<exists> y z. x1 = (ANil, y, z) \<and> x2 = ANil) \<or>
+                    (\<exists>subst subst_assn as y z v e.
+                        x1 = (ACons v e as, y, z) \<and>
+                        x2 = (ACons v (subst (e, y, z)) (subst_assn (as, y, z))) \<and>
+                        fst p ((e, y, z)) ((subst (e, y, z))) \<and>
+                        snd p ((as, y, z)) ((subst_assn (as, y, z))))
+   ))
+)"
+
+
+definition conv where
+  "conv \<equiv> (\<lambda> fp. (\<lambda> x1 x2. sum_case (\<lambda> x1. sum_case (\<lambda> x2. fst fp x1 x2) (\<lambda> x2. False) x2) (\<lambda> x1. (sum_case (\<lambda> x2. False) (\<lambda> x2. snd fp x1 x2) x2)) x1))"
+
+lemma substAltEnc2:"
+lfp f2  = conv (lfp f3)"
+oops
+
+lemma sumC_rewrite:
+ "(\<lambda>x. THE_default undefined (lfp f1 x)) = 
+  (sum_case (\<lambda>x1 . Inl (THE_default undefined (fst (lfp f3) x1)))
+            (\<lambda>x2 . Inr (THE_default undefined (snd (lfp f3) x2))))"
+oops
+*)
+
+(* Helper lemmas provided by Christian Urban *)
+
+lemma Projl_permute:
+  assumes a: "\<exists>y. f = Inl y"
+  shows "(p \<bullet> (Sum_Type.Projl f)) = Sum_Type.Projl (p \<bullet> f)"
+using a by auto
+
+lemma Projr_permute:
+  assumes a: "\<exists>y. f = Inr y"
+  shows "(p \<bullet> (Sum_Type.Projr f)) = Sum_Type.Projr (p \<bullet> f)"
+using a by auto
+
+nominal_primrec  (default "sum_case (\<lambda>x. Inl undefined) (\<lambda>x. Inr undefined)",
+                  invariant "\<lambda> a r . (\<forall> as y z . ((a = Inr (as, y, z) \<and> set (bn as) \<sharp>* (y, z)) \<longrightarrow> bn (Sum_Type.Projr r) = bn as))")
+  subst :: "exp \<Rightarrow> var \<Rightarrow> var \<Rightarrow> exp" ("_[_::=_]" [1000,100,100] 1000)
+and
+  subst_assn :: "assn \<Rightarrow> var \<Rightarrow> var \<Rightarrow> assn"
+where
+  "(Var x)[y ::= z] = (Var (x[y ::v= z]))"
+ |"(App e v)[y ::= z] = (App (e[y ::= z]) (v[y ::v= z]))"
+ |"(set (bn as)) \<sharp>* (y,z) \<Longrightarrow> (Let as body)[y ::= z] = Let (subst_assn as y z) (body[y ::= z])" 
+ |"(atom x \<sharp> (y,z)) \<Longrightarrow> (Lam [x].e)[y ::= z] = Lam [x].(e[y::=z])"
+ |"subst_assn ANil y z = ANil"
+ |"subst_assn (ACons v e as) y z = ACons v (e[y ::= z]) (subst_assn as y z)"
+proof-
+
+have eqvt_at_subst: "\<And> e y z . eqvt_at subst_subst_assn_sumC (Inl (e, y, z)) \<Longrightarrow> eqvt_at (\<lambda>(a, b, c). subst a b c) (e, y, z)"
+  apply(simp add: eqvt_at_def subst_def)
+  apply(rule)
+  apply(subst Projl_permute)
+  apply(thin_tac "?X")+
+  apply (simp add: subst_subst_assn_sumC_def)
+  apply (simp add: THE_default_def)
+  apply (case_tac "Ex1 (subst_subst_assn_graph (Inl (e, y, z)))")
+  apply(simp)
+  apply(auto)[1]
+  apply (erule_tac x="x" in allE)
+  apply simp
+  apply(cases rule: subst_subst_assn_graph.cases)
+  apply(assumption)
+  apply(rule_tac x="Sum_Type.Projl x" in exI)
+  apply(clarify)
+  apply (rule the1_equality)
+  apply blast 
+  apply(simp (no_asm) only: Projl.simps)
+  apply(rule_tac x="Sum_Type.Projl x" in exI)
+  apply(clarify)
+  apply (rule the1_equality)
+  apply blast 
+  apply(simp (no_asm) only: Projl.simps)
+  apply(rule_tac x="Sum_Type.Projl x" in exI)
+  apply(clarify)
+  apply (rule the1_equality)
+  apply blast 
+  apply(simp (no_asm) only: Projl.simps)
+  apply(rule_tac x="Sum_Type.Projl x" in exI)
+  apply(clarify)
+  apply (rule the1_equality)
+  apply blast 
+  apply(simp (no_asm) only: Projl.simps)
+  apply (metis Inr_not_Inl)
+  apply (metis Inr_not_Inl)
+  apply(simp)
+  apply(perm_simp)
+  apply(simp)
+done
+
+have eqvt_at_subst_assn: "\<And> as y z . eqvt_at subst_subst_assn_sumC (Inr (as, y, z)) \<Longrightarrow> eqvt_at (\<lambda>(a, b, c). subst_assn a b c) (as, y, z)"
+  apply(simp add: eqvt_at_def subst_assn_def)
+  apply(rule)
+  apply(subst Projr_permute)
+  apply(thin_tac "?X")+
+  apply (simp add: subst_subst_assn_sumC_def)
+  apply (simp add: THE_default_def)
+  apply (case_tac "Ex1 (subst_subst_assn_graph (Inr (as, y, z)))")
+  apply(simp)
+  apply(auto)[1]
+  apply (erule_tac x="x" in allE)
+  apply simp
+  apply(cases rule: subst_subst_assn_graph.cases)
+  apply(assumption)
+  apply (metis Inr_not_Inl)+
+  apply(rule_tac x="Sum_Type.Projr x" in exI)
+  apply(clarify)
+  apply (rule the1_equality)
+  apply auto[1]
+  apply(simp (no_asm) only: Projr.simps)
+  
+  apply(rule_tac x="Sum_Type.Projr x" in exI)
+  apply(clarify)
+  apply (rule the1_equality)
+  apply auto[1]
+  apply(simp (no_asm) only: Projr.simps)
+  
+  apply(simp)
+  apply(perm_simp)
+  apply(simp)
+done
+
+{
+(* Equivariance of the graph *)
+case goal1 thus ?case
+  unfolding eqvt_def subst_subst_assn_graph_def
+  apply(subst (1 2) substAltDef[unfolded f1_def f2_def]) 
+  apply(rule)
+  apply perm_simp
+  apply rule
+done
+
+(* The invariant *)
+next case goal2 thus ?case
+  by (induct rule: subst_subst_assn_graph.induct)(auto simp add: exp_assn.bn_defs fresh_star_insert)
+
+(* Exhaustiveness *)
+next case (goal3 P x) show ?case
+  proof(cases x)
+  case (Inl a) thus P
+    proof(cases a)
+    case (fields a1 a2 a3)
+    thus P using Inl goal3
+      apply (rule_tac y ="a1" and c ="(a2, a3)" in exp_assn.strong_exhaust(1))
+      apply (auto simp add: fresh_star_def)
+    done
+  qed
+  next
+  case (Inr a) thus P
+    proof (cases a)
+    case (fields a1 a2 a3)
+    thus P using Inr goal3
+      apply (rule_tac ya ="a1" in exp_assn.strong_exhaust(2))
+      apply (auto)
+      apply blast+
+    done
+  qed
+qed
+
+next case (goal15 e y2 z2 as e2 y z as2) thus ?case
+  apply -
+  apply (drule eqvt_at_subst)+
+  apply (drule eqvt_at_subst_assn)+
+  apply (simp only: meta_eq_to_obj_eq[OF subst_def, symmetric, unfolded fun_eq_iff]
+    meta_eq_to_obj_eq[OF subst_assn_def, symmetric, unfolded fun_eq_iff])
+  (* No _sum any more at this point! *)
+  apply (auto simp add: Abs_fresh_iff)
+  apply (drule_tac
+    c = "(y, z)" and
+    as = "(bn e)" and
+    bs = "(bn e2)" and
+    f = "\<lambda> a b c . [a]lst. (subst (fst b) y z, subst_assn (snd b) y z )" in Abs_lst_fcb2)
+  apply (auto simp add: perm_supp_eq fresh_Pair fresh_star_def Abs_fresh_iff eqvt_at_def)
+  done
+
+next case (goal19 x2 y2 z2 e2 x y z e) thus ?case
+  apply -
+  apply (drule eqvt_at_subst)+
+  apply (simp only: Abs_fresh_iff meta_eq_to_obj_eq[OF subst_def, symmetric, unfolded fun_eq_iff])
+  (* No _sum any more at this point! *)
+  apply (auto)
+  apply (erule_tac c = "(y, z)" in Abs_lst_fcb2)
+  apply (auto simp add: perm_supp_eq fresh_Pair fresh_star_def Abs_fresh_iff eqvt_at_def)
+  done
+}
+qed(auto)
+
+termination (eqvt) by lexicographic_order
+
+nominal_primrec vars_as
+where
+  "vars_as ANil = {}"
+ |"vars_as (ACons v e as) = insert v (vars_as as)"
+apply(simp add: eqvt_def vars_as_graph_def)
+apply(rule, perm_simp, rule)
+apply auto[1]
+apply(case_tac x rule: exp_assn.exhaust(2))
+apply auto
+done
+termination (eqvt) by lexicographic_order
+
+nominal_primrec frees and frees_as
+where
+  "frees (Var x) = {x}"
+ |"frees (App e x) = insert x (frees e)"
+ |"frees (Lam [x]. e) = (frees e) - {x}"
+ |"frees (Let as body) = (frees body \<union> frees_as as) - (vars_as as)"
+ |"frees_as ANil = {}"
+ |"frees_as (ACons v e as) = frees e \<union> frees_as as"
+apply(simp add: eqvt_def frees_frees_as_graph_def)
+apply(rule, perm_simp, rule)
+apply auto[1]
+
+apply(case_tac x)
+apply(case_tac a rule: exp_assn.exhaust(1))
+apply auto[4]
+apply(case_tac b rule: exp_assn.exhaust(2))
+apply auto[2]
+apply auto[1]
+apply auto[1]
+apply auto[1]
+apply auto[1]
+apply auto[1]
+apply auto[1]
+apply auto[1]
+apply auto[1]
+apply auto[1]
+apply auto[1]
+apply auto[1]
+
+sorry
+termination (eqvt) by lexicographic_order
+
+lemma shows
+  True and bn_subst[simp]: "set (bn as) \<sharp>* (y, z) \<Longrightarrow> bn (subst_assn as y z) = bn as"
+by(induct rule:subst_subst_assn.induct)
+  (auto simp add: exp_assn.bn_defs fresh_star_insert)
+
+abbreviation
+  LetBe :: "var\<Rightarrow>exp\<Rightarrow>exp\<Rightarrow>exp" ("let _ be _ in _ " [100,100,100] 100)
+where
+  "let x be t1 in t2 \<equiv> Let (ACons x t1 ANil) t2"
+              
+lemma alpha_test:
+  shows "Lam [x]. (Var x) = Lam [y]. (Var y)"
+  by (simp add: exp_assn.eq_iff Abs1_eq_iff exp_assn.fresh fresh_at_base)
+
+lemma alpha_test2:
+  shows "let x be (Var x) in (Var x) = let y be (Var y) in (Var y)"
+  by (simp add:exp_assn.eq_iff exp_assn.bn_defs Abs1_eq_iff fresh_Pair add:exp_assn.fresh fresh_at_base)
+
+lemma alpha_test3:
+  shows "
+    Let (ACons x (Var y) (ACons y (Var x) ANil)) (Var x)
+    =
+    Let (ACons y (Var x) (ACons x (Var y) ANil)) (Var y)" (is "Let ?la ?lb = _")
+  apply (simp add:exp_assn.eq_iff exp_assn.bn_defs Abs1_eq_iff fresh_Pair add:exp_assn.fresh fresh_at_base)
+  apply (simp add: Abs_swap2[of "atom x" "(?lb,?la)" "[atom x, atom y]" "atom y"])
+done
+
+end
